\documentclass[answers]{exam}
\usepackage{texPreamble}
\usepackage{relsize}
\usepackage{tabularx}
\extraheadheight{0.25in}
\extrafootheight{1.0in}
\extrawidth{1in}
% ----------------------------------------------------------------
\makeatletter
\title{Summary on Briggs 3.9:\\Derivatives of Logarithmic and Exponential Functions}
%\date{}

\pagestyle{headandfoot}
\firstpageheader{\@date}{\@title}{}
\firstpageheadrule

\runningfootrule
\runningfooter{}{\thepage\ / \numpages}{\@title}
\makeatother

\firstpagefootrule
\runningfootrule
\begin{document}
\begin{enumerate}
  \item Make sure you're using the correct rule:
    \begin{center}
      \begin{tabular}{@{}LcR@{}}\toprule
        \textnormal{Function}& Derivative rule& \textnormal{Example}\\\midrule
        c^b& Constant& \ds\ddx\sbrkt{\pi^{e}}=0\\[12.5:pt]
        x^c& Power& \ds\ddx\sbrkt{x^3}=3x^2\\[12.5:pt]
        c^x& Exponent& \ds\ddx\sbrkt{c^x}=\ln(c)\, c^x\\[12.5:pt]
        \log_b(x)& Logarithm& \ds\ddx\sbrkt{\log_2(x)}=\ddx\sbrkt{\frac{\ln(x)}{\ln(2)}}=\frac{1}{\ln(2) x}
        \\\bottomrule
      \end{tabular}
    \end{center}
  \item Make sure you're familiar with the laws of logarithms! Simplifying before taking a derivative can make the problem much easier!!
    \begin{align*}
      &\hspace*{-15pt}\ddx\sbrkt{\ln\parens{\frac{(42x^2+1:)^2(33x-15)^3(110x\inv-1)^4}{(2x+7)^3\cos(x)e^{\inv[x]}}}}\\
      &=\ddx\sbrkt{2\ln(42x^2+1:)+3\ln(33x-15)+4\ln(110x\inv-1)-3\ln(2x+7)-\ln(\cos(x))+x}\\
      &=2\frac{84x}{42x^2+1:}+3\frac{33}{33x-15}+4\frac{-110x\inv[2]}{110x\inv-1}-3\frac{2}{2x+7}-\frac{-\sin(x)}{\cos(x)}+1
    \end{align*}
  \item 
    Logarithmic differentiation can be used to ``break apart'' functions of the form $f(x)^{g(x)}$. Notice that this is when the base AND the exponent of the function contain a variable:
      \begin{align*}
        f(x)=(3x^2+1:)^{\cos(x)}&\Rightarrow \ln(f(x))=\ln\parens{(3x^2+1)^{\cos(x)}}\\
          &\Rightarrow \ln(f(x))=\cos(x)\ln\parens{3x^2+1:}\\
        \intertext{The next step uses chain rule on the left-hand side and product rule on the right:}
          &\Rightarrow \frac{1}{f(x)}f'(x)=\ddx\sbrkt{\cos(x)}\ln\parens{3x^2+1:}+\cos(x)\ddx\sbrkt{\ln\parens{3x^2+1}}\\
        \intertext{Use the derivative of $\cos(x)$ and $\ln(f(x))$ (chain-rule)}
          &\Rightarrow \frac{f'(x)}{f(x)}=-\sin(x)\ln\parens{3x^2+1:}+\cos(x)\frac{1}{3x^2+1}\cdot\ddx\sbrkt{3x^2+1}\\
          &\Rightarrow \frac{f'(x)}{f(x)}=-\sin(x)\ln\parens{3x^2+1:}+\cos(x)\frac{6x}{3x^2+1}\\
        \intertext{Since the original function was only in terms of $x$, we need to write the derivative solely in terms of $x$. We do this by multiplying both sides by $f(x)$ and then substituting the original function back in:}
          &\Rightarrow f'(x)=f(x)\parens{-\sin(x)\ln\parens{3x^2+1:}+\cos(x)\frac{6x}{3x^2+1}}\\
         &\Rightarrow \boxed{f'(x)=\parens{3x^2+1:}^{\cos(x)}\parens{-\sin(x)\ln\parens{3x^2+1}+\cos(x)\frac{6x}{3x^2+1}}}
      \end{align*}
  \item 
    MyLab Math has examples where you can rewrite a function using $e^x$ and $\ln(x)$. This method is equivalent:
      \begin{align*}
        f(x)&=\parens{3x^2+1:}^{\cos(x)}=e^{\ln\parens{\parens{3x^2+1}^{\cos(x)}}}=e^{\cos(x)\ln\parens{3x^2+1}}\\
        f'(x)&=e^{\cos(x)\ln\parens{3x^2+1:}}\ddx\sbrkt{\cos(x)\ln\parens{3x^2+1}}\\
        f'(x)&=e^{\cos(x)\ln\parens{3x^2+1:}}\parens{\ddx\sbrkt{\cos(x)}\ln\parens{3x^2+1}+\cos(x)\ddx\sbrkt{\ln\parens{3x^2+1}}}\\
        f'(x)&=e^{\cos(x)\ln\parens{3x^2+1:}}\parens{-\sin(x)\ln\parens{3x^2+1}+\cos(x)\frac{6x}{3x^2+1}}\\
        f'(x)&=\parens{3x^2+1:}^{\cos(x)}\parens{-\sin(x)\ln\parens{3x^2+1}+\cos(x)\frac{6x}{3x^2+1}}
      \end{align*}
\end{enumerate}
\end{document}